Structure/Generic/Categories.lean
@@ -1,16 +1,16 @@
---  An abstract formalization of "isomorphism is equality up to relabeling"
--- -------------------------------------------------------------------------
---
--- See `README.md` for more info.
---
--- This file contains definitions of (potentially higher) categories and groupoids.
-
-
-
 import Structure.Generic.Axioms
+import Structure.Generic.Instances.Basic
+import Structure.Generic.Instances.Bundled
 import Structure.Generic.Functors
 
+open GeneralizedRelation
 
+
+
+-- TODO: Are we overthinking this? Should we maybe just define that a _universe_ is a category/groupoid, with its instance arrows/equivalences?
+-- HasMorphisms extends HasFunctorialArrows
+-- HasIsomorphisms extends HasFunctorialEquivalences
+-- But what about real-life categories that are not universes?
 
 section Categories
 
@@ -46,15 +46,113 @@ section BundledCategories
 
   variable (M : Universe) [HasInternalFunctors M] [HasInstanceArrows M]
 
-  @[reducible] def Category := Bundled (IsCategory M)
-  @[reducible] def Groupoid := Bundled (IsGroupoid M)
+  namespace IsCategory
+
+    @[reducible] def Category := Bundled (IsCategory M)
+
+    @[reducible] def category : Universe := bundledUniverse (U := sortUniverse) (IsCategory M)
+
+    instance (S : category M) : IsCategory M ⌈S⌉ := bundledInstance (U := sortUniverse) (IsCategory M) S
+
+  end IsCategory
+
+  namespace IsGroupoid
+
+    @[reducible] def Groupoid := Bundled (IsGroupoid M)
+
+    @[reducible] def groupoid : Universe := bundledUniverse (U := sortUniverse) (IsGroupoid M)
+
+    instance (S : groupoid M) : IsGroupoid M ⌈S⌉ := bundledInstance (U := sortUniverse) (IsGroupoid M) S
+
+  end IsGroupoid
 
 end BundledCategories
 
 
 
+section ExternalFunctors
+
+  variable (M : Universe) [HasInternalFunctors M] [HasInstanceArrows M]
+           (N : Universe) [HasInternalFunctors N] [HasInstanceArrows N]
+           [HasExternalFunctors M N]
+
+  namespace IsCategory
+
+    instance hasFunctoriality : Bundled.HasFunctoriality (IsCategory M) (IsCategory N) := ⟨IsArrowFunctor M N⟩
+
+    instance {S : category M} {T : category N} (F : S ⟶' T) : IsArrowFunctor M N F.f := F.isFun
+
+  end IsCategory
+
+  namespace IsGroupoid
+
+    instance hasFunctoriality : Bundled.HasFunctoriality (IsGroupoid M) (IsGroupoid N) := ⟨IsEquivFunctor M N⟩
+
+    instance {S : groupoid M} {T : groupoid N} (F : S ⟶' T) : IsEquivFunctor M N F.f := F.isFun
+
+  end IsGroupoid
+
+end ExternalFunctors
+
+
+
+section InternalFunctors
+
+  variable (M : Universe) [HasInternalFunctors M] [HasInstanceEquivalences M] [hNat : HasNaturalQuantification sortUniverse sortUniverse M M]
+
+  namespace IsCategory
+
+    -- TODO
+
+  end IsCategory
+
+  namespace IsGroupoid
+
+    def Equiv {S T : groupoid M} (F G : S ⟶' T) := NaturalEquivalence M M F.f G.f
+
+    -- TODO: Can we write this more cleanly?
+    def EquivRel (S T : groupoid M) : GeneralizedRelation (S ⟶' T) M :=
+    λ F G => (hNat.hasNat S.inst.Equiv T.inst.Equiv
+                          (h := T.inst.isEquiv.toHasTrans)
+                          (mF := HasInternalFunctors.toBundled F.f) (mG := HasInternalFunctors.toBundled G.f)
+                          F.isFun.mapEquiv G.isFun.mapEquiv).Nat (h := T.inst.isEquiv.toHasTrans)
+
+    instance functorGroupoid (S T : groupoid M) : IsGroupoid M (S ⟶' T) :=
+    { Equiv   := EquivRel M (hNat := hNat) S T,
+      isEquiv := sorry,
+      isIso   := sorry }
+
+    instance hasFunctorInstances : Bundled.HasFunctorInstances (IsGroupoid M) := ⟨functorGroupoid M (hNat := hNat)⟩
+
+    --instance hasInternalFunctors : HasInternalFunctors (groupoid M) := Bundled.hasInternalFunctors (IsGroupoid M)
+  
+  end IsGroupoid
+
+end InternalFunctors
+
+
+
+section ExternalFunctorOperations
+
+  section idFun
+
+    variable (M : Universe) [HasInternalFunctors M] [HasInstanceArrows M] [HasIdFun M]
+
+    instance IsCategory.hasIdFun : HasIdFun (category M) := ⟨λ _ => idFun.isArrowFunctor M⟩
+    instance IsGroupoid.hasIdFun : HasIdFun (groupoid M) := ⟨λ _ => idFun.isEquivFunctor M⟩
+
+  end idFun
+
+  -- TODO: constFun, compFun
+
+end ExternalFunctorOperations
+
+
+
 -- TODO: Show that:
 -- * the universes of categories and groupoids have nice properties
---   (-> bundled functors -> natural transformation as equivalence -> internal functors), and
+--   (-> bundled functors -> natural transformation as equivalence -> internal functors, also instance arrows/equivalences), and
 -- * universes with certain properties are actually categories/groupoids
 --   (-> category of categories, groupoid of groupoids).
+-- TODO: At some point, we will add the assumption that the `Equiv` relation of a universe has isomorphisms.
+-- So all instances are groupoids. How does that fit into this scheme?
