Structure/Generic/Instances/Basic.lean
@@ -1,0 +1,184 @@
+import Structure.Generic.Axioms
+
+import mathlib4_experiments.CoreExt
+
+open GeneralizedRelation
+
+
+
+set_option autoBoundImplicitLocal false
+--set_option pp.universes true
+
+universes u v w
+
+
+
+def sortUniverse : Universe.{u, u + 1} := ⟨Sort u⟩
+@[reducible] def propUniverse := sortUniverse.{0}
+@[reducible] def typeUniverse := sortUniverse.{u + 1}
+
+namespace SortUniverse
+
+  instance hasExternalFunctors : HasExternalFunctors sortUniverse.{u} sortUniverse.{v} := ⟨λ _ => True⟩
+
+  def funEquiv (α β : sortUniverse.{u}) : (α → β) ≃ (α ⟶' β) :=
+  { toFun    := λ f      => ⟨f, trivial⟩,
+    invFun   := λ F      => F.f,
+    leftInv  := λ _      => rfl,
+    rightInv := λ ⟨_, _⟩ => rfl }
+
+  instance hasInternalFunctors : HasInternalFunctors sortUniverse.{u} :=
+  { Fun      := λ α β => α → β,
+    funEquiv := funEquiv }
+
+  instance hasIdFun    : HasIdFun    sortUniverse.{u}                                   := ⟨λ _     => trivial⟩
+  instance hasConstFun : HasConstFun sortUniverse.{u} sortUniverse.{v}                  := ⟨λ _ _ _ => trivial⟩
+  instance hasCompFun  : HasCompFun  sortUniverse.{u} sortUniverse.{v} sortUniverse.{w} := ⟨λ _ _   => trivial⟩
+
+  instance hasFunOp : HasFunOp sortUniverse.{u} :=
+  { constFunIsFun   := λ _ _   => trivial,
+    appIsFun        := λ _ _   => trivial,
+    appFunIsFun     := λ _ _   => trivial,
+    dupIsFun        := λ _     => trivial,
+    dupFunIsFun     := λ _ _   => trivial,
+    compFunIsFun    := λ _ _   => trivial,
+    compFunFunIsFun := λ _ _ _ => trivial }
+
+end SortUniverse
+
+
+
+def UnivRel (α : Sort u) : GeneralizedRelation α propUniverse := λ _ _ => True
+
+def UnivRel.isEquivalence {α : Sort u} : Equivalence (UnivRel α) :=
+⟨λ _ => trivial, λ _ => trivial, λ _ _ => trivial⟩
+
+namespace GeneralizedRelation.IsEquivalence
+
+  -- Every equivalence relation can trivially be converted to an instance of `IsEquivalence`.
+  instance relEquiv {α : Sort u} {R : GeneralizedRelation α propUniverse} (e : Equivalence R) : IsEquivalence R :=
+  { refl  := e.refl,
+    symm  := e.symm,
+    trans := e.trans }
+
+  -- So these are the instances that we obtain directly from Lean.
+  instance univ   (α : Sort u)                : IsEquivalence (V := propUniverse) (UnivRel α) := relEquiv UnivRel.isEquivalence
+  instance iff                                : IsEquivalence (V := propUniverse) Iff         := relEquiv Iff.isEquivalence
+  instance eq     (α : Sort u)                : IsEquivalence (V := propUniverse) (@Eq α)     := relEquiv Eq.isEquivalence
+  instance setoid (α : Sort u) [s : Setoid α] : IsEquivalence (V := propUniverse) s.r         := relEquiv s.iseqv
+
+end GeneralizedRelation.IsEquivalence
+
+
+
+-- TODO: Convert products, `Iff`, and `Equiv` to general axioms and an instance similar to `Fun` -> `Arrow`.
+
+namespace HasProducts
+
+  instance : HasSymm (V := propUniverse) And := ⟨λ h => ⟨h.right, h.left⟩⟩
+  instance : HasProducts Prop propUniverse := ⟨And⟩
+
+  instance : HasSymm (V := typeUniverse.{u}) Prod := ⟨λ p => ⟨p.snd, p.fst⟩⟩
+  instance : HasProducts (Type u) typeUniverse.{u} := ⟨Prod⟩
+
+end HasProducts
+
+namespace HasEquivalences
+
+  def univ   (α : Sort u)                : HasEquivalences α    propUniverse := ⟨UnivRel α⟩
+  instance iff                           : HasEquivalences Prop propUniverse := ⟨Iff⟩
+  def eq     (α : Sort u)                : HasEquivalences α    propUniverse := ⟨Eq⟩
+  def setoid (α : Sort u) [s : Setoid α] : HasEquivalences α    propUniverse := ⟨s.r⟩
+
+end HasEquivalences
+
+
+
+namespace HasInstanceEquivalences
+
+  -- By specializing here, we avoid invoking proof irrelevance explicitly.
+  -- Instead, we just declare all proofs to be equivalent according to our own notion of equivalence.
+  instance prop : HasInstanceEquivalences propUniverse     := ⟨propUniverse, UnivRel⟩
+  instance type : HasInstanceEquivalences typeUniverse.{u} := ⟨propUniverse, @Eq⟩
+
+  instance : HasInstanceArrows propUniverse     := HasInstanceEquivalences.toHasInstanceArrows propUniverse
+  instance : HasInstanceArrows typeUniverse.{u} := HasInstanceEquivalences.toHasInstanceArrows typeUniverse.{u}
+
+end HasInstanceEquivalences
+
+namespace HasFunctorialEquivalences
+
+  instance prop : HasFunctorialEquivalences propUniverse :=
+  { equivCongr := λ _ _ => trivial }
+
+  instance type : HasFunctorialEquivalences typeUniverse.{u} :=
+  { equivCongr := congr }
+
+end HasFunctorialEquivalences
+
+
+
+namespace PropRel
+
+  section Morphisms
+
+    variable {α : Sort u} (R : GeneralizedRelation α propUniverse) [IsEquivalence R]
+
+    instance isCompositionRelation : IsCompositionRelation R :=
+    { assocLR := λ _ _ _ => trivial,
+      assocRL := λ _ _ _ => trivial }
+
+    instance isMorphismRelation : IsMorphismRelation R :=
+    { leftId  := λ _ => trivial,
+      rightId := λ _ => trivial }
+
+    instance isIsomorphismRelation : IsIsomorphismRelation R :=
+    { leftInv  := λ _   => trivial,
+      rightInv := λ _   => trivial,
+      invInv   := λ _   => trivial,
+      compInv  := λ _ _ => trivial,
+      idInv    := λ _   => trivial }
+
+  end Morphisms
+
+  section Functors
+
+    variable {α : Sort u} {V : Universe} [HasInternalFunctors V] [HasExternalFunctors V propUniverse]
+             (R : GeneralizedRelation α V) (S : GeneralizedRelation α propUniverse)
+             [IsEquivalence R] [IsEquivalence S]
+             (F : BaseFunctor R S)
+
+    instance isReflFunctor  : IsReflFunctor  R S F := ⟨λ _   => trivial⟩
+    instance isSymmFunctor  : IsSymmFunctor  R S F := ⟨λ _   => trivial⟩
+    instance isTransFunctor : IsTransFunctor R S F := ⟨λ _ _ => trivial⟩
+
+    instance isPreorderFunctor    : IsPreorderFunctor    R S F := ⟨⟩
+    instance isEquivalenceFunctor : IsEquivalenceFunctor R S F := ⟨⟩
+
+  end Functors
+
+  section NaturalTransformations
+
+    variable {α : Sort u} {β : Sort v} {V : Universe} [HasInternalFunctors V] [HasExternalFunctors V propUniverse]
+             (R : GeneralizedRelation α V) (S : GeneralizedRelation β propUniverse) [HasTrans S]
+             {mF mG : α → β} (F : MappedBaseFunctor R S mF) (G : MappedBaseFunctor R S mG)
+
+    instance isNatural (n : ∀ a, S (mF a) (mG a)) : IsNatural R S F G n := ⟨λ _ => trivial⟩
+
+    def natEquiv : (∀ a, S (mF a) (mG a)) ≃ NaturalQuantification R S F G :=
+    { toFun    := λ n => ⟨n⟩,
+      invFun   := λ N => N.n,
+      leftInv  := λ _ => rfl,
+      rightInv := λ { n := _, isNatural := ⟨_⟩ } => rfl }
+
+    instance hasIntNat : HasInternalNaturalQuantification R S F G :=
+    { Nat      := ∀ a, S (mF a) (mG a),
+      natEquiv := natEquiv R S F G }
+
+  end NaturalTransformations
+
+  instance hasNat {U₁ U₂ V : Universe} [HasExternalFunctors U₁ U₂] [HasExternalFunctors V propUniverse] :
+    HasNaturalQuantification U₁ U₂ V propUniverse :=
+  { hasNat := λ {α β} R S {h mF mG} F G => hasIntNat R S F G }
+
+end PropRel
