Structure/Generic/Instances/BundledSetoid.lean
@@ -1,0 +1,84 @@
+import Structure.Generic.Axioms
+import Structure.Generic.Instances.Bundled
+
+
+
+set_option autoBoundImplicitLocal false
+--set_option pp.universes true
+
+universes u v w
+
+
+
+def BundledSetoid := Bundled Setoid
+@[reducible] def bundledSetoid : Universe := bundledUniverse (U := typeUniverse.{u}) Setoid
+
+namespace BundledSetoid
+
+  instance isSetoid (S : bundledSetoid) : Setoid ⌈S⌉ := S.inst
+  instance (S : bundledSetoid) : Setoid ⌈S⌉ := isSetoid S
+
+  class IsFunctorial {S T : bundledSetoid} (f : S → T) where
+  (mapEquiv {a b : S} : a ≈ b → f a ≈ f b)
+
+  instance hasFunctoriality : Bundled.HasFunctoriality.{u + 1, u + 1, v + 1, v + 1, 1} Setoid Setoid := ⟨IsFunctorial⟩
+
+  namespace BundledFunctor
+
+    theorem congrArg {S T : bundledSetoid} (F : S ⟶' T) {a b : S} : a ≈ b → F a ≈ F b := F.isFun.mapEquiv
+
+    def Equiv {S T : bundledSetoid} (F G : S ⟶' T) := ∀ a, F a ≈ G a
+
+    namespace Equiv
+
+      variable {S T : bundledSetoid}
+
+      theorem refl  (F     : S ⟶' T)                                 : Equiv F F := λ a => Setoid.refl  (F a)
+      theorem symm  {F G   : S ⟶' T} (h : Equiv F G)                 : Equiv G F := λ a => Setoid.symm  (h a)
+      theorem trans {F G H : S ⟶' T} (h : Equiv F G) (i : Equiv G H) : Equiv F H := λ a => Setoid.trans (h a) (i a)
+
+      def isEquivalence : Equivalence (@Equiv S T) := ⟨refl, symm, trans⟩
+
+    end Equiv
+
+    instance isSetoid (S T : bundledSetoid) : Setoid (S ⟶' T) := ⟨Equiv, Equiv.isEquivalence⟩
+
+    theorem congrFun {S T : bundledSetoid} {F G : S ⟶' T} (h : F ≈ G) (a : S) : F a ≈ G a := h a
+
+    theorem congr {S T : bundledSetoid} {F G : S ⟶' T} {a b : S} : F ≈ G → a ≈ b → F a ≈ G b :=
+    λ h₁ h₂ => Setoid.trans (congrFun h₁ a) (congrArg G h₂)
+
+    instance hasFunctorInstances : Bundled.HasFunctorInstances.{u + 1, u + 1, 1} Setoid := ⟨isSetoid⟩
+
+  end BundledFunctor
+
+  instance hasInternalFunctors : HasInternalFunctors bundledSetoid := Bundled.hasInternalFunctors Setoid
+
+  instance hasIdFun    : HasIdFun    bundledSetoid.{u}                                     :=
+  ⟨λ S           => ⟨id⟩⟩
+  instance hasConstFun : HasConstFun bundledSetoid.{u} bundledSetoid.{v}                   :=
+  ⟨λ S {T}   c   => ⟨Function.const _ (Setoid.refl c)⟩⟩
+  instance hasCompFun  : HasCompFun  bundledSetoid.{u} bundledSetoid.{v} bundledSetoid.{w} :=
+  ⟨λ {S T U} F G => ⟨G.isFun.mapEquiv ∘ F.isFun.mapEquiv⟩⟩
+
+  instance hasInstanceEquivalences : HasInstanceEquivalences bundledSetoid :=
+  ⟨propUniverse, λ S => (isSetoid S).r⟩
+
+  instance hasFunctorialEquivalences : HasFunctorialEquivalences bundledSetoid :=
+  { equivCongr := BundledFunctor.congr }
+
+  -- TODO: Move to `Bundled.lean`
+  instance hasFunOp : HasFunOp bundledSetoid :=
+  { constFunIsFun   := λ S T       => ⟨λ hc a   => hc⟩,
+    appIsFun        := λ {S} a T   => ⟨λ hF     => BundledFunctor.congrFun hF a⟩,
+    appFunIsFun     := λ S T       => ⟨λ ha F   => BundledFunctor.congrArg F ha⟩,
+    dupIsFun        := λ {S T} F   => ⟨λ ha     => BundledFunctor.congr (BundledFunctor.congrArg F ha) ha⟩,
+    dupFunIsFun     := λ S T       => ⟨λ hF a   => BundledFunctor.congrFun (BundledFunctor.congrFun hF a) a⟩,
+    compFunIsFun    := λ {S T} F U => ⟨λ hG a   => BundledFunctor.congrFun hG (F a)⟩,
+    compFunFunIsFun := λ S T U     => ⟨λ hF G a => BundledFunctor.congrArg G (BundledFunctor.congrFun hF a)⟩ }
+
+  def eq (α : Sort u) : BundledSetoid :=
+  { α    := α,
+    inst := ⟨Eq, Eq.isEquivalence⟩ }
+
+end BundledSetoid
