Structure/Generic/Instances/Equiv.lean
@@ -1,0 +1,46 @@
+import Structure.Generic.Axioms
+import Structure.Generic.Instances.Basic
+
+import mathlib4_experiments.Data.Equiv.Basic
+
+open GeneralizedRelation
+
+
+
+set_option autoBoundImplicitLocal false
+--set_option pp.universes true
+
+universes u
+
+
+
+def EquivRel : GeneralizedRelation (Type u) typeUniverse.{u} := Equiv
+
+namespace EquivRel
+
+  -- TODO: We want to use this to show that `typeUniverse` is a groupoid, along with `propUniverse` and `groupoid` itself.
+  -- See bottom of `Categories.lean`.
+
+  instance isEquivalence : IsEquivalence EquivRel :=
+  { refl  := Equiv.refl,
+    symm  := Equiv.symm,
+    trans := Equiv.trans }
+
+  instance isCompositionRelation : IsCompositionRelation EquivRel :=
+  { assocLR := λ f g h => Eq.symm (Equiv.trans_assoc f g h),
+    assocRL := Equiv.trans_assoc }
+
+  instance isMorphismRelation : IsMorphismRelation EquivRel :=
+  { leftId  := Equiv.trans_refl,
+    rightId := Equiv.refl_trans }
+
+  instance isIsomorphismRelation : IsIsomorphismRelation EquivRel :=
+  { leftInv  := Equiv.trans_symm,
+    rightInv := Equiv.symm_trans,
+    invInv   := Equiv.symm_symm,
+    compInv  := Equiv.symm_trans_symm,
+    idInv    := @Equiv.refl_symm }
+
+end EquivRel
+
+instance typeHasEquivalences : HasEquivalences (Type u) typeUniverse.{u} := ⟨EquivRel⟩
