Structure/Generic/Lemmas.lean
@@ -1,12 +1,3 @@
---  An abstract formalization of "isomorphism is equality up to relabeling"
--- -------------------------------------------------------------------------
---
--- See `README.md` for more info.
---
--- Lemmas following from axioms in `Axioms.lean`.
-
-
-
 import Structure.Generic.Axioms
 import mathlib4_experiments.Data.Equiv.Basic
 
@@ -38,11 +29,11 @@ namespace HasFunOp
   def swapIsFun {α β γ : U} (F : α ⟶' β ⟶ γ) (b : β) : HasExternalFunctors.IsFun (λ a : α => F a b) :=
   h.compIsFun F (appFun' b γ)
 
-  def swapFun' {α β γ : U} (F : α ⟶' β ⟶ γ) (b : β) : α ⟶' γ := HasInternalFunctors.mkFun' (swapIsFun F                                 b)
-  def swapFun  {α β γ : U} (F : α ⟶  β ⟶ γ) (b : β) : α ⟶  γ := HasInternalFunctors.mkFun  (swapIsFun (HasInternalFunctors.toBundled F) b)
+  def swapFun' {α β γ : U} (F : α ⟶' β ⟶ γ) (b : β) : α ⟶' γ := BundledFunctor.mkFun      (swapIsFun F                                 b)
+  def swapFun  {α β γ : U} (F : α ⟶  β ⟶ γ) (b : β) : α ⟶  γ := HasInternalFunctors.mkFun (swapIsFun (HasInternalFunctors.toBundled F) b)
 
   @[simp] theorem swapFun.eff {α β γ : U} (F : α ⟶ β ⟶ γ) (b : β) (a : α) :
-    (swapFun F b) a = F⟮a⟯ b :=
+    (swapFun F b) a = F a b :=
   by apply HasInternalFunctors.mkFun.eff
 
   theorem swapFunFun.def {α β γ : U} (F : α ⟶' β ⟶ γ) (b : β) :
@@ -52,11 +43,11 @@ namespace HasFunOp
   def swapFunIsFun {α β γ : U} (F : α ⟶' β ⟶ γ) : HasExternalFunctors.IsFun (λ b : β => HasInternalFunctors.mkFun (swapIsFun F b)) :=
   funext (swapFunFun.def F) ▸ h.compIsFun (appFunFun' β γ) (compFunFun' F γ)
 
-  def swapFunFun' {α β γ : U} (F : α ⟶' β ⟶ γ) : β ⟶' α ⟶ γ := HasInternalFunctors.mkFun' (swapFunIsFun F)
-  def swapFunFun  {α β γ : U} (F : α ⟶  β ⟶ γ) : β ⟶  α ⟶ γ := HasInternalFunctors.mkFun  (swapFunIsFun (HasInternalFunctors.toBundled F))
+  def swapFunFun' {α β γ : U} (F : α ⟶' β ⟶ γ) : β ⟶' α ⟶ γ := BundledFunctor.mkFun      (swapFunIsFun F)
+  def swapFunFun  {α β γ : U} (F : α ⟶  β ⟶ γ) : β ⟶  α ⟶ γ := HasInternalFunctors.mkFun (swapFunIsFun (HasInternalFunctors.toBundled F))
 
   @[simp] theorem swapFunFun.eff {α β γ : U} (F : α ⟶ β ⟶ γ) (b : β) :
-    (swapFunFun F)⟮b⟯ = swapFun F b :=
+    (swapFunFun F) b = swapFun F b :=
   by apply HasInternalFunctors.mkFun.eff
 
   theorem swapFunFunFun.def (α β γ : U) (F : α ⟶ β ⟶ γ) :
@@ -67,18 +58,18 @@ namespace HasFunOp
   funext (swapFunFunFun.def α β γ) ▸ h.compIsFun (compFunFunFun' α (β ⟶ γ) γ)
                                                  (compFunFun' (appFunFun' β γ) (α ⟶ γ))
 
-  def swapFunFunFun' (α β γ : U) : (α ⟶ β ⟶ γ) ⟶' (β ⟶ α ⟶ γ) := HasInternalFunctors.mkFun' (swapFunFunIsFun α β γ)
-  def swapFunFunFun  (α β γ : U) : (α ⟶ β ⟶ γ) ⟶  (β ⟶ α ⟶ γ) := HasInternalFunctors.mkFun  (swapFunFunIsFun α β γ)
+  def swapFunFunFun' (α β γ : U) : (α ⟶ β ⟶ γ) ⟶' (β ⟶ α ⟶ γ) := BundledFunctor.mkFun      (swapFunFunIsFun α β γ)
+  def swapFunFunFun  (α β γ : U) : (α ⟶ β ⟶ γ) ⟶  (β ⟶ α ⟶ γ) := HasInternalFunctors.mkFun (swapFunFunIsFun α β γ)
 
   @[simp] theorem swapFunFunFun.eff (α β γ : U) (F : α ⟶ β ⟶ γ) :
-    (swapFunFunFun α β γ)⟮F⟯ = swapFunFun F :=
+    (swapFunFunFun α β γ) F = swapFunFun F :=
   by apply HasInternalFunctors.mkFun.eff
 
   -- In particular, reverse composition is also functorial.
 
   theorem revCompFunFun.def (α : U) {β γ : U} (G : β ⟶' γ) (F : α ⟶ β) :
-    HasInternalFunctors.mkFun (h.compIsFun (HasInternalFunctors.toBundled F) G) = (compFunFun F γ)⟮HasInternalFunctors.fromBundled G⟯ :=
-  Eq.subst (motive := λ H => HasInternalFunctors.mkFun (h.compIsFun (HasInternalFunctors.toBundled F) H) = (compFunFun F γ)⟮HasInternalFunctors.fromBundled G⟯)
+    HasInternalFunctors.mkFun (h.compIsFun (HasInternalFunctors.toBundled F) G) = (compFunFun F γ) (HasInternalFunctors.fromBundled G) :=
+  Eq.subst (motive := λ H => HasInternalFunctors.mkFun (h.compIsFun (HasInternalFunctors.toBundled F) H) = (compFunFun F γ) (HasInternalFunctors.fromBundled G))
            (HasInternalFunctors.toFromBundled G)
            (Eq.symm (compFunFun.eff F γ (HasInternalFunctors.fromBundled G)))
 
@@ -86,11 +77,11 @@ namespace HasFunOp
     HasExternalFunctors.IsFun (λ F : α ⟶ β => HasInternalFunctors.mkFun (h.compIsFun (HasInternalFunctors.toBundled F) G)) :=
   funext (revCompFunFun.def α G) ▸ swapIsFun (compFunFunFun' α β γ) (HasInternalFunctors.fromBundled G)
 
-  def revCompFunFun' (α : U) {β γ : U} (G : β ⟶' γ) : (α ⟶ β) ⟶' (α ⟶ γ) := HasInternalFunctors.mkFun' (revCompFunIsFun α G)
-  def revCompFunFun  (α : U) {β γ : U} (G : β ⟶  γ) : (α ⟶ β) ⟶  (α ⟶ γ) := HasInternalFunctors.mkFun  (revCompFunIsFun α (HasInternalFunctors.toBundled G))
+  def revCompFunFun' (α : U) {β γ : U} (G : β ⟶' γ) : (α ⟶ β) ⟶' (α ⟶ γ) := BundledFunctor.mkFun      (revCompFunIsFun α G)
+  def revCompFunFun  (α : U) {β γ : U} (G : β ⟶  γ) : (α ⟶ β) ⟶  (α ⟶ γ) := HasInternalFunctors.mkFun (revCompFunIsFun α (HasInternalFunctors.toBundled G))
 
   @[simp] theorem revCompFunFun.eff (α : U) {β γ : U} (G : β ⟶ γ) (F : α ⟶ β) :
-    (revCompFunFun α G)⟮F⟯ = G ⊙ F :=
+    (revCompFunFun α G) F = G ⊙ F :=
   by apply HasInternalFunctors.mkFun.eff
 
   theorem revCompFunFunFun.def (α β γ : U) (G : β ⟶ γ) :
@@ -101,11 +92,11 @@ namespace HasFunOp
     HasExternalFunctors.IsFun (λ G : β ⟶ γ => revCompFunFun α G) :=
   funext (revCompFunFunFun.def α β γ) ▸ swapFunIsFun (compFunFunFun' α β γ)
 
-  def revCompFunFunFun' (α β γ : U) : (β ⟶ γ) ⟶' (α ⟶ β) ⟶ (α ⟶ γ) := HasInternalFunctors.mkFun' (revCompFunFunIsFun α β γ)
-  def revCompFunFunFun  (α β γ : U) : (β ⟶ γ) ⟶  (α ⟶ β) ⟶ (α ⟶ γ) := HasInternalFunctors.mkFun  (revCompFunFunIsFun α β γ)
+  def revCompFunFunFun' (α β γ : U) : (β ⟶ γ) ⟶' (α ⟶ β) ⟶ (α ⟶ γ) := BundledFunctor.mkFun      (revCompFunFunIsFun α β γ)
+  def revCompFunFunFun  (α β γ : U) : (β ⟶ γ) ⟶  (α ⟶ β) ⟶ (α ⟶ γ) := HasInternalFunctors.mkFun (revCompFunFunIsFun α β γ)
 
   @[simp] theorem revCompFunFunFun.eff (α β γ : U) (G : β ⟶ γ) :
-    (revCompFunFunFun α β γ)⟮G⟯ = revCompFunFun α G :=
+    (revCompFunFunFun α β γ) G = revCompFunFun α G :=
   by apply HasInternalFunctors.mkFun.eff
 
   -- Composition of a function with two arguments.
@@ -123,11 +114,11 @@ namespace HasFunOp
   def substIsFun {α β γ : U} (F : α ⟶' β ⟶ γ) (G : α ⟶' β) : HasExternalFunctors.IsFun (λ a : α => F a (G a)) :=
   funext (substFun.def F G) ▸ h.dupIsFun (swapFunFun' F ⊙' G)
 
-  def substFun' {α β γ : U} (F : α ⟶' β ⟶ γ) (G : α ⟶' β) : α ⟶' γ := HasInternalFunctors.mkFun' (substIsFun F                    G)
-  def substFun  {α β γ : U} (F : α ⟶  β ⟶ γ) (G : α ⟶  β) : α ⟶  γ := HasInternalFunctors.mkFun  (substIsFun (HasInternalFunctors.toBundled F) (HasInternalFunctors.toBundled G))
+  def substFun' {α β γ : U} (F : α ⟶' β ⟶ γ) (G : α ⟶' β) : α ⟶' γ := BundledFunctor.mkFun      (substIsFun F                    G)
+  def substFun  {α β γ : U} (F : α ⟶  β ⟶ γ) (G : α ⟶  β) : α ⟶  γ := HasInternalFunctors.mkFun (substIsFun (HasInternalFunctors.toBundled F) (HasInternalFunctors.toBundled G))
 
   @[simp] theorem substFun.eff {α β γ : U} (F : α ⟶ β ⟶ γ) (G : α ⟶ β) (a : α) :
-    (substFun F G) a = F⟮a⟯ (G a) :=
+    (substFun F G) a = F a (G a) :=
   by apply HasInternalFunctors.mkFun.eff
 
   theorem substFunFun.def {α β γ : U} (F : α ⟶' β ⟶ γ) (G : α ⟶ β) :
@@ -139,11 +130,11 @@ namespace HasFunOp
     HasExternalFunctors.IsFun (λ G : α ⟶ β => HasInternalFunctors.mkFun (substIsFun F (HasInternalFunctors.toBundled G))) :=
   funext (substFunFun.def F) ▸ h.compIsFun (revCompFunFun' α (swapFunFun' F)) (dupFunFun' α γ)
 
-  def substFunFun' {α β γ : U} (F : α ⟶' β ⟶ γ) : (α ⟶ β) ⟶' (α ⟶ γ) := HasInternalFunctors.mkFun' (substFunIsFun F)
-  def substFunFun  {α β γ : U} (F : α ⟶  β ⟶ γ) : (α ⟶ β) ⟶  (α ⟶ γ) := HasInternalFunctors.mkFun  (substFunIsFun (HasInternalFunctors.toBundled F))
+  def substFunFun' {α β γ : U} (F : α ⟶' β ⟶ γ) : (α ⟶ β) ⟶' (α ⟶ γ) := BundledFunctor.mkFun      (substFunIsFun F)
+  def substFunFun  {α β γ : U} (F : α ⟶  β ⟶ γ) : (α ⟶ β) ⟶  (α ⟶ γ) := HasInternalFunctors.mkFun (substFunIsFun (HasInternalFunctors.toBundled F))
 
   @[simp] theorem substFunFun.eff {α β γ : U} (F : α ⟶ β ⟶ γ) (G : α ⟶ β) :
-    (substFunFun F)⟮G⟯ = substFun F G :=
+    (substFunFun F) G = substFun F G :=
   by apply HasInternalFunctors.mkFun.eff
 
   theorem substFunFunFun.def (α β γ : U) (F : α ⟶ β ⟶ γ) :
@@ -154,11 +145,11 @@ namespace HasFunOp
   funext (substFunFunFun.def α β γ) ▸ h.compIsFun (revCompFunFunFun' α β (α ⟶ γ) ⊙' swapFunFunFun' α β γ)
                                                   (revCompFunFun' (α ⟶ β) (dupFunFun' α γ))
 
-  def substFunFunFun' (α β γ : U) : (α ⟶ β ⟶ γ) ⟶' (α ⟶ β) ⟶ (α ⟶ γ) := HasInternalFunctors.mkFun' (substFunFunIsFun α β γ)
-  def substFunFunFun  (α β γ : U) : (α ⟶ β ⟶ γ) ⟶  (α ⟶ β) ⟶ (α ⟶ γ) := HasInternalFunctors.mkFun  (substFunFunIsFun α β γ)
+  def substFunFunFun' (α β γ : U) : (α ⟶ β ⟶ γ) ⟶' (α ⟶ β) ⟶ (α ⟶ γ) := BundledFunctor.mkFun      (substFunFunIsFun α β γ)
+  def substFunFunFun  (α β γ : U) : (α ⟶ β ⟶ γ) ⟶  (α ⟶ β) ⟶ (α ⟶ γ) := HasInternalFunctors.mkFun (substFunFunIsFun α β γ)
 
   @[simp] theorem substFunFunFun.eff (α β γ : U) (F : α ⟶ β ⟶ γ) :
-    (substFunFunFun α β γ)⟮F⟯ = substFunFun F :=
+    (substFunFunFun α β γ) F = substFunFun F :=
   by apply HasInternalFunctors.mkFun.eff
 
 
@@ -260,10 +251,8 @@ namespace HasFunctorialArrows
 
   variable (U : Universe) [HasInternalFunctors U] [h : HasFunctorialArrows U]
 
-  def arrowCongrArg  {α β : U} (F : α ⟶{U} β) {a b : α} : (a ⇝ b) ⟶{h.arrowUniverse} (F a ⇝ F b) := h.arrowCongr⟮HasRefl.refl F⟯
-  def arrowCongrArg' {α β : U} (F : α ⟶'   β) {a b : α} : (a ⇝ b) ⟶{h.arrowUniverse} (F a ⇝ F b) := HasInternalFunctors.fromBundled.coe F ▸ arrowCongrArg U (HasInternalFunctors.fromBundled F)
-
-  def arrowCongrFun {α β : U} {F G : α ⟶{U} β} (a : α) : (F ⇝ G) ⟶{h.arrowUniverse} (F a ⇝ G a) := HasFunOp.swapFun h.arrowCongr (HasRefl.refl a)
+  def arrow_congrFun  {α β : U} {F G : α ⟶ β} (a : α) : (F ⇝ G) ⟶ (F a ⇝ G a) := HasFunOp.swapFun h.arrowCongr (HasRefl.refl a)
+  def arrow_congrFun' {α β : U} {F G : α ⟶ β} (a : α) : (F ⇝ G) → (F a ⇝ G a) := HasInternalFunctors.funCoe (arrow_congrFun U a)
 
 end HasFunctorialArrows
 
@@ -271,10 +260,8 @@ namespace HasFunctorialEquivalences
 
   variable (U : Universe) [HasInternalFunctors U] [h : HasFunctorialEquivalences U]
 
-  def equivCongrArg  {α β : U} (F : α ⟶{U} β) {a b : α} : a ≃ b ⟶{h.equivUniverse} F a ≃ F b := h.equivCongr⟮HasRefl.refl F⟯
-  def equivCongrArg' {α β : U} (F : α ⟶'   β) {a b : α} : a ≃ b ⟶{h.equivUniverse} F a ≃ F b := HasInternalFunctors.fromBundled.coe F ▸ equivCongrArg U (HasInternalFunctors.fromBundled F)
-
-  def equivCongrFun {α β : U} {F G : α ⟶{U} β} (a : α) : F ≃ G ⟶{h.equivUniverse} F a ≃ G a := HasFunOp.swapFun h.equivCongr (HasRefl.refl a)
+  def equiv_congrFun  {α β : U} {F G : α ⟶ β} (a : α) : F ≃ G ⟶ F a ≃ G a := HasFunOp.swapFun h.equivCongr (HasRefl.refl a)
+  def equiv_congrFun' {α β : U} {F G : α ⟶ β} (a : α) : F ≃ G → F a ≃ G a := HasInternalFunctors.funCoe (equiv_congrFun U a)
 
 end HasFunctorialEquivalences
 
@@ -286,7 +273,7 @@ structure Iff' {U : Universe} [HasInternalFunctors U] (α β : U) where
 (mp  : α ⟶ β)
 (mpr : β ⟶ α)
 
-notation:20 α:21 " ⟷{" U':0 "} " β:21 => Iff' (U := U') α β
+infix:20 " ⟷' " => Iff'
 
 
 
@@ -302,44 +289,44 @@ section Morphisms
 
     variable [HasTrans R] [IsCompositionRelation R]
 
-    def comp_congrArg {a b c : α} {f₁ f₂ : R a b} {g₁ g₂ : R b c} : f₁ ≃ f₂ ⟶{he.equivUniverse} g₁ ≃ g₂ ⟶ g₁ • f₁ ≃ g₂ • f₂ :=
-    he.equivCongr ⊙ HasFunctorialEquivalences.equivCongrArg U HasTrans.trans
+    def comp_congrArg {a b c : α} {f₁ f₂ : R a b} {g₁ g₂ : R b c} : f₁ ≃ f₂ ⟶ g₁ ≃ g₂ ⟶ g₁ • f₁ ≃ g₂ • f₂ :=
+    he.equivCongr ⊙ HasFunctorialEquivalences.equiv_congrArg U HasTrans.trans
 
-    def comp_congrArg_left  {a b c : α} {f : R a b} {g₁ g₂ : R b c} : g₁ ≃ g₂ ⟶{he.equivUniverse} g₁ • f ≃ g₂ • f :=
-    HasFunctorialEquivalences.equivCongrArg U (HasTrans.trans'' f)
+    def comp_congrArg_left  {a b c : α} {f : R a b} {g₁ g₂ : R b c} : g₁ ≃ g₂ ⟶ g₁ • f ≃ g₂ • f :=
+    HasFunctorialEquivalences.equiv_congrArg U (HasTrans.trans ⟮f⟯)
 
-    def comp_congrArg_right {a b c : α} {f₁ f₂ : R a b} {g : R b c} : f₁ ≃ f₂ ⟶{he.equivUniverse} g • f₁ ≃ g • f₂ :=
+    def comp_congrArg_right {a b c : α} {f₁ f₂ : R a b} {g : R b c} : f₁ ≃ f₂ ⟶ g • f₁ ≃ g • f₂ :=
     HasFunOp.swapFun comp_congrArg (HasRefl.refl g)
 
-    def comp_subst  {a b c : α} {f₁ f₂ : R a b} {g₁ g₂ : R b c} {e : R a c} : f₁ ≃ f₂ ⟶{he.equivUniverse} g₁ ≃ g₂ ⟶ g₂ • f₂ ≃ e ⟶ g₁ • f₁ ≃ e :=
+    def comp_subst  {a b c : α} {f₁ f₂ : R a b} {g₁ g₂ : R b c} {e : R a c} : f₁ ≃ f₂ ⟶ g₁ ≃ g₂ ⟶ g₂ • f₂ ≃ e ⟶ g₁ • f₁ ≃ e :=
     HasFunOp.compFun₂ comp_congrArg HasTrans.trans
-    def comp_subst' {a b c : α} {f₁ f₂ : R a b} {g₁ g₂ : R b c} {e : R a c} : f₁ ≃ f₂ ⟶{he.equivUniverse} g₁ ≃ g₂ ⟶ e ≃ g₁ • f₁ ⟶ e ≃ g₂ • f₂ :=
+    def comp_subst' {a b c : α} {f₁ f₂ : R a b} {g₁ g₂ : R b c} {e : R a c} : f₁ ≃ f₂ ⟶ g₁ ≃ g₂ ⟶ e ≃ g₁ • f₁ ⟶ e ≃ g₂ • f₂ :=
     HasFunOp.compFun₂ comp_congrArg HasTrans.revTrans
 
-    def comp_subst_left   {a b c : α} (f : R a b) {g₁ g₂ : R b c} {e : R a c} : g₁ ≃ g₂ ⟶{he.equivUniverse} g₂ • f ≃ e ⟶ g₁ • f ≃ e :=
+    def comp_subst_left   {a b c : α} (f : R a b) {g₁ g₂ : R b c} {e : R a c} : g₁ ≃ g₂ ⟶ g₂ • f ≃ e ⟶ g₁ • f ≃ e :=
     HasTrans.trans    ⊙ comp_congrArg_left
-    def comp_subst_left'  {a b c : α} (f : R a b) {g₁ g₂ : R b c} {e : R a c} : g₁ ≃ g₂ ⟶{he.equivUniverse} e ≃ g₁ • f ⟶ e ≃ g₂ • f :=
+    def comp_subst_left'  {a b c : α} (f : R a b) {g₁ g₂ : R b c} {e : R a c} : g₁ ≃ g₂ ⟶ e ≃ g₁ • f ⟶ e ≃ g₂ • f :=
     HasTrans.revTrans ⊙ comp_congrArg_left
 
-    def comp_subst_right  {a b c : α} {f₁ f₂ : R a b} (g : R b c) {e : R a c} : f₁ ≃ f₂ ⟶{he.equivUniverse} g • f₂ ≃ e ⟶ g • f₁ ≃ e :=
+    def comp_subst_right  {a b c : α} {f₁ f₂ : R a b} (g : R b c) {e : R a c} : f₁ ≃ f₂ ⟶ g • f₂ ≃ e ⟶ g • f₁ ≃ e :=
     HasTrans.trans    ⊙ comp_congrArg_right
-    def comp_subst_right' {a b c : α} {f₁ f₂ : R a b} (g : R b c) {e : R a c} : f₁ ≃ f₂ ⟶{he.equivUniverse} e ≃ g • f₁ ⟶ e ≃ g • f₂ :=
+    def comp_subst_right' {a b c : α} {f₁ f₂ : R a b} (g : R b c) {e : R a c} : f₁ ≃ f₂ ⟶ e ≃ g • f₁ ⟶ e ≃ g • f₂ :=
     HasTrans.revTrans ⊙ comp_congrArg_right
 
-    def applyAssocLR_left  {a b c d : α} {f : R a b} {g : R b c} {h : R c d} {e : R a d} : (h • g) • f ≃ e ⟶{he.equivUniverse} h • (g • f) ≃ e :=
-    HasTrans.trans'' (assocRL f g h)
-    def applyAssocRL_left  {a b c d : α} {f : R a b} {g : R b c} {h : R c d} {e : R a d} : h • (g • f) ≃ e ⟶{he.equivUniverse} (h • g) • f ≃ e :=
-    HasTrans.trans'' (assocLR f g h)
-    def applyAssocLR_right {a b c d : α} {f : R a b} {g : R b c} {h : R c d} {e : R a d} : e ≃ (h • g) • f ⟶{he.equivUniverse} e ≃ h • (g • f) :=
+    def applyAssocLR_left  {a b c d : α} {f : R a b} {g : R b c} {h : R c d} {e : R a d} : (h • g) • f ≃ e ⟶ h • (g • f) ≃ e :=
+    HasTrans.trans ⟮assocRL f g h⟯
+    def applyAssocRL_left  {a b c d : α} {f : R a b} {g : R b c} {h : R c d} {e : R a d} : h • (g • f) ≃ e ⟶ (h • g) • f ≃ e :=
+    HasTrans.trans ⟮assocLR f g h⟯
+    def applyAssocLR_right {a b c d : α} {f : R a b} {g : R b c} {h : R c d} {e : R a d} : e ≃ (h • g) • f ⟶ e ≃ h • (g • f) :=
     HasTrans.revTrans'' (assocLR f g h)
-    def applyAssocRL_right {a b c d : α} {f : R a b} {g : R b c} {h : R c d} {e : R a d} : e ≃ h • (g • f) ⟶{he.equivUniverse} e ≃ (h • g) • f :=
+    def applyAssocRL_right {a b c d : α} {f : R a b} {g : R b c} {h : R c d} {e : R a d} : e ≃ h • (g • f) ⟶ e ≃ (h • g) • f :=
     HasTrans.revTrans'' (assocRL f g h)
 
     def applyAssocLR {a β₁ β₂ γ₁ γ₂ d : α} {f₁ : R a β₁} {f₂ : R a β₂} {g₁ : R β₁ γ₁} {g₂ : R β₂ γ₂} {h₁ : R γ₁ d} {h₂ : R γ₂ d} :
-      (h₁ • g₁) • f₁ ≃ (h₂ • g₂) • f₂ ⟶{he.equivUniverse} h₁ • (g₁ • f₁) ≃ h₂ • (g₂ • f₂) :=
+      (h₁ • g₁) • f₁ ≃ (h₂ • g₂) • f₂ ⟶ h₁ • (g₁ • f₁) ≃ h₂ • (g₂ • f₂) :=
     applyAssocLR_right ⊙ applyAssocLR_left
     def applyAssocRL {a β₁ β₂ γ₁ γ₂ d : α} {f₁ : R a β₁} {f₂ : R a β₂} {g₁ : R β₁ γ₁} {g₂ : R β₂ γ₂} {h₁ : R γ₁ d} {h₂ : R γ₂ d} :
-      h₁ • (g₁ • f₁) ≃ h₂ • (g₂ • f₂) ⟶{he.equivUniverse} (h₁ • g₁) • f₁ ≃ (h₂ • g₂) • f₂ :=
+      h₁ • (g₁ • f₁) ≃ h₂ • (g₂ • f₂) ⟶ (h₁ • g₁) • f₁ ≃ (h₂ • g₂) • f₂ :=
     applyAssocRL_right ⊙ applyAssocRL_left
 
   end IsCompositionRelation
@@ -348,9 +335,9 @@ section Morphisms
 
     variable [IsPreorder R] [IsMorphismRelation R]
 
-    def leftCancelId  {a b : α} (f : R a b) {e : R b b} : e ≃ ident R b ⟶{he.equivUniverse} e • f ≃ f :=
+    def leftCancelId  {a b : α} (f : R a b) {e : R b b} : e ≃ ident R b ⟶ e • f ≃ f :=
     HasFunOp.swapFun (comp_subst_left  f) (leftId  f)
-    def rightCancelId {a b : α} (f : R a b) {e : R a a} : e ≃ ident R a ⟶{he.equivUniverse} f • e ≃ f :=
+    def rightCancelId {a b : α} (f : R a b) {e : R a a} : e ≃ ident R a ⟶ f • e ≃ f :=
     HasFunOp.swapFun (comp_subst_right f) (rightId f)
 
   end IsMorphismRelation
@@ -361,61 +348,61 @@ section Morphisms
 
     variable [IsEquivalence R] [IsIsomorphismRelation R]
 
-    def inv_congrArg {a b : α} {f₁ f₂ : R a b} : f₁ ≃ f₂ ⟶{he.equivUniverse} f₁⁻¹ ≃ f₂⁻¹ :=
-    HasFunctorialEquivalences.equivCongrArg U HasSymm.symm
+    def inv_congrArg {a b : α} {f₁ f₂ : R a b} : f₁ ≃ f₂ ⟶ f₁⁻¹ ≃ f₂⁻¹ :=
+    HasFunctorialEquivalences.equiv_congrArg U HasSymm.symm
 
-    def inv_subst  {a b : α} {f₁ f₂ : R a b} {e : R b a} : f₁ ≃ f₂ ⟶{he.equivUniverse} f₂⁻¹ ≃ e ⟶ f₁⁻¹ ≃ e :=
+    def inv_subst  {a b : α} {f₁ f₂ : R a b} {e : R b a} : f₁ ≃ f₂ ⟶ f₂⁻¹ ≃ e ⟶ f₁⁻¹ ≃ e :=
     HasTrans.trans    ⊙ inv_congrArg
-    def inv_subst' {a b : α} {f₁ f₂ : R a b} {e : R b a} : f₁ ≃ f₂ ⟶{he.equivUniverse} e ≃ f₁⁻¹ ⟶ e ≃ f₂⁻¹ :=
+    def inv_subst' {a b : α} {f₁ f₂ : R a b} {e : R b a} : f₁ ≃ f₂ ⟶ e ≃ f₁⁻¹ ⟶ e ≃ f₂⁻¹ :=
     HasTrans.revTrans ⊙ inv_congrArg
 
-    def leftCancel'     {a b c : α} (f : R a b) (g : R b c) : (g⁻¹ • g) • f ≃ f := (leftCancelId  f)⟮leftInv  g⟯
-    def leftCancel      {a b c : α} (f : R a b) (g : R b c) : g⁻¹ • (g • f) ≃ f := applyAssocLR_left⟮leftCancel'     f g⟯
-    def leftCancelInv'  {a b c : α} (f : R a b) (g : R c b) : (g • g⁻¹) • f ≃ f := (leftCancelId  f)⟮rightInv g⟯
-    def leftCancelInv   {a b c : α} (f : R a b) (g : R c b) : g • (g⁻¹ • f) ≃ f := applyAssocLR_left⟮leftCancelInv'  f g⟯
-    def rightCancel'    {a b c : α} (f : R a b) (g : R c a) : f • (g • g⁻¹) ≃ f := (rightCancelId f)⟮rightInv g⟯
-    def rightCancel     {a b c : α} (f : R a b) (g : R c a) : (f • g) • g⁻¹ ≃ f := applyAssocRL_left⟮rightCancel'    f g⟯
-    def rightCancelInv' {a b c : α} (f : R a b) (g : R a c) : f • (g⁻¹ • g) ≃ f := (rightCancelId f)⟮leftInv  g⟯
-    def rightCancelInv  {a b c : α} (f : R a b) (g : R a c) : (f • g⁻¹) • g ≃ f := applyAssocRL_left⟮rightCancelInv' f g⟯
+    def leftCancel'     {a b c : α} (f : R a b) (g : R b c) : (g⁻¹ • g) • f ≃ f := (leftCancelId  f) (leftInv  g)
+    def leftCancel      {a b c : α} (f : R a b) (g : R b c) : g⁻¹ • (g • f) ≃ f := applyAssocLR_left ⟮leftCancel'     f g⟯
+    def leftCancelInv'  {a b c : α} (f : R a b) (g : R c b) : (g • g⁻¹) • f ≃ f := (leftCancelId  f) (rightInv g)
+    def leftCancelInv   {a b c : α} (f : R a b) (g : R c b) : g • (g⁻¹ • f) ≃ f := applyAssocLR_left ⟮leftCancelInv'  f g⟯
+    def rightCancel'    {a b c : α} (f : R a b) (g : R c a) : f • (g • g⁻¹) ≃ f := (rightCancelId f) (rightInv g)
+    def rightCancel     {a b c : α} (f : R a b) (g : R c a) : (f • g) • g⁻¹ ≃ f := applyAssocRL_left ⟮rightCancel'    f g⟯
+    def rightCancelInv' {a b c : α} (f : R a b) (g : R a c) : f • (g⁻¹ • g) ≃ f := (rightCancelId f) (leftInv  g)
+    def rightCancelInv  {a b c : α} (f : R a b) (g : R a c) : (f • g⁻¹) • g ≃ f := applyAssocRL_left ⟮rightCancelInv' f g⟯
 
-    def leftMulInv  {a b c : α} (f₁ : R a b) (f₂ : R a c) (g : R b c) : g • f₁ ≃ f₂ ⟷{he.equivUniverse} f₁ ≃ g⁻¹ • f₂ :=
+    def leftMulInv  {a b c : α} (f₁ : R a b) (f₂ : R a c) (g : R b c) : g • f₁ ≃ f₂ ⟷' f₁ ≃ g⁻¹ • f₂ :=
     ⟨HasFunOp.swapFun (comp_subst_right' g⁻¹) (HasSymm.symm' (leftCancel f₁ g)),
      HasFunOp.swapFun (comp_subst_right  g)   (leftCancelInv f₂ g)⟩
-    def leftMulInv' {a b c : α} (f₁ : R a b) (f₂ : R a c) (g : R c b) : g⁻¹ • f₁ ≃ f₂ ⟷{he.equivUniverse} f₁ ≃ g • f₂ :=
+    def leftMulInv' {a b c : α} (f₁ : R a b) (f₂ : R a c) (g : R c b) : g⁻¹ • f₁ ≃ f₂ ⟷' f₁ ≃ g • f₂ :=
     ⟨HasFunOp.swapFun (comp_subst_right' g)   (HasSymm.symm' (leftCancelInv f₁ g)),
      HasFunOp.swapFun (comp_subst_right  g⁻¹) (leftCancel f₂ g)⟩
 
-    def leftMul {a b c : α} (f₁ f₂ : R a b) (g : R b c) : g • f₁ ≃ g • f₂ ⟷{he.equivUniverse} f₁ ≃ f₂ :=
+    def leftMul {a b c : α} (f₁ f₂ : R a b) (g : R b c) : g • f₁ ≃ g • f₂ ⟷' f₁ ≃ f₂ :=
     ⟨HasTrans.revTrans'' (leftCancel f₂ g) ⊙ (leftMulInv f₁ (g • f₂) g).mp, comp_congrArg_right⟩
 
-    def rightMulInv  {a b c : α} (f₁ : R a c) (f₂ : R b c) (g : R b a) : f₁ • g ≃ f₂ ⟷{he.equivUniverse} f₁ ≃ f₂ • g⁻¹ :=
+    def rightMulInv  {a b c : α} (f₁ : R a c) (f₂ : R b c) (g : R b a) : f₁ • g ≃ f₂ ⟷' f₁ ≃ f₂ • g⁻¹ :=
     ⟨HasFunOp.swapFun (comp_subst_left' g⁻¹) (HasSymm.symm' (rightCancel f₁ g)),
      HasFunOp.swapFun (comp_subst_left  g)   (rightCancelInv f₂ g)⟩
-    def rightMulInv' {a b c : α} (f₁ : R a c) (f₂ : R b c) (g : R a b) : f₁ • g⁻¹ ≃ f₂ ⟷{he.equivUniverse} f₁ ≃ f₂ • g :=
+    def rightMulInv' {a b c : α} (f₁ : R a c) (f₂ : R b c) (g : R a b) : f₁ • g⁻¹ ≃ f₂ ⟷' f₁ ≃ f₂ • g :=
     ⟨HasFunOp.swapFun (comp_subst_left' g)   (HasSymm.symm' (rightCancelInv f₁ g)),
      HasFunOp.swapFun (comp_subst_left  g⁻¹) (rightCancel f₂ g)⟩
 
-    def rightMul {a b c : α} (f₁ f₂ : R a b) (g : R c a) : f₁ • g ≃ f₂ • g ⟷{he.equivUniverse} f₁ ≃ f₂ :=
+    def rightMul {a b c : α} (f₁ f₂ : R a b) (g : R c a) : f₁ • g ≃ f₂ • g ⟷' f₁ ≃ f₂ :=
     ⟨HasTrans.revTrans'' (rightCancel f₂ g) ⊙ (rightMulInv f₁ (f₂ • g) g).mp, comp_congrArg_left⟩
 
-    def eqInvIffInvEq {a b : α} (f : R a b) (g : R b a) : f ≃ g⁻¹ ⟷{he.equivUniverse} f⁻¹ ≃ g :=
+    def eqInvIffInvEq {a b : α} (f : R a b) (g : R b a) : f ≃ g⁻¹ ⟷' f⁻¹ ≃ g :=
     ⟨HasFunOp.swapFun inv_subst  (invInv g),
      HasFunOp.swapFun inv_subst' (HasSymm.symm' (invInv f))⟩
 
-    def eqIffEqInv {a b : α} (f₁ f₂ : R a b) : f₁⁻¹ ≃ f₂⁻¹ ⟷{he.equivUniverse} f₁ ≃ f₂ :=
+    def eqIffEqInv {a b : α} (f₁ f₂ : R a b) : f₁⁻¹ ≃ f₂⁻¹ ⟷' f₁ ≃ f₂ :=
     ⟨HasTrans.revTrans'' (invInv f₂) ⊙ (eqInvIffInvEq f₁ f₂⁻¹).mpr, inv_congrArg⟩
 
     def leftRightMul {a b c d : α} (f₁ : R a b) (f₂ : R a c) (g₁ : R b d) (g₂ : R c d) :
-      g₂⁻¹ • g₁ ≃ f₂ • f₁⁻¹ ⟷{he.equivUniverse} g₁ • f₁ ≃ g₂ • f₂ :=
+      g₂⁻¹ • g₁ ≃ f₂ • f₁⁻¹ ⟷' g₁ • f₁ ≃ g₂ • f₂ :=
     ⟨(leftMulInv' (g₁ • f₁) f₂ g₂).mp ⊙ applyAssocLR_left ⊙ (rightMulInv (g₂⁻¹ • g₁) f₂ f₁).mpr,
      (leftMulInv' g₁ (f₂ • f₁⁻¹) g₂).mpr ⊙ applyAssocLR_right ⊙ (rightMulInv g₁ (g₂ • f₂) f₁).mp⟩
 
     def swapInv  {a b c d : α} (f₁ : R a b) (f₂ : R c d) (g₁ : R d b) (g₂ : R c a) :
-      g₁⁻¹ • f₁ ≃ f₂ • g₂⁻¹ ⟶{he.equivUniverse} f₁⁻¹ • g₁ ≃ g₂ • f₂⁻¹ :=
+      g₁⁻¹ • f₁ ≃ f₂ • g₂⁻¹ ⟶ f₁⁻¹ • g₁ ≃ g₂ • f₂⁻¹ :=
     (leftRightMul f₂ g₂ g₁ f₁).mpr ⊙ HasSymm.symm ⊙ (leftRightMul g₂ f₂ f₁ g₁).mp
 
     def swapInv' {a b c d : α} (f₁ : R a b) (f₂ : R c d) (g₁ : R d b) (g₂ : R c a) :
-      f₂ • g₂⁻¹ ≃ g₁⁻¹ • f₁ ⟶{he.equivUniverse} g₂ • f₂⁻¹ ≃ f₁⁻¹ • g₁ :=
+      f₂ • g₂⁻¹ ≃ g₁⁻¹ • f₁ ⟶ g₂ • f₂⁻¹ ≃ f₁⁻¹ • g₁ :=
     HasSymm.symm ⊙ swapInv f₁ f₂ g₁ g₂ ⊙ HasSymm.symm
 
   end IsIsomorphismRelation
@@ -428,65 +415,77 @@ end Morphisms
 
 section Functors
 
-  variable {α : Sort u} {U : Universe} [HasFunOp U] [hasArrows : HasFunctorialArrows U]
+  variable {α : Sort u}
 
   namespace idFun
 
-    variable (R : GeneralizedRelation α U)
+    variable {U : Universe} [HasInstanceArrows U] [HasExternalFunctors U U]
+             [HasIdFun U] (R : GeneralizedRelation α U)
 
-    instance isReflFunctor  [HasRefl  R] : IsReflFunctor  R R (HasFunOp.idFun' _) :=
+    instance isReflFunctor  [HasRefl  R] : IsReflFunctor  R R (HasIdFun.idFun' _) :=
     ⟨λ a   => HasRefl.refl (ident R a)⟩
 
-    instance isSymmFunctor  [HasSymm  R] : IsSymmFunctor  R R (HasFunOp.idFun' _) :=
+    variable [HasInternalFunctors U]
+
+    instance isSymmFunctor  [HasSymm  R] : IsSymmFunctor  R R (HasIdFun.idFun' _) :=
     ⟨λ f   => HasRefl.refl f⁻¹⟩
 
-    instance isTransFunctor [HasTrans R] : IsTransFunctor R R (HasFunOp.idFun' _) :=
+    instance isTransFunctor [HasTrans R] : IsTransFunctor R R (HasIdFun.idFun' _) :=
     ⟨λ f g => HasRefl.refl (g • f)⟩
 
-    instance isPreorderFunctor    [IsPreorder    R] : IsPreorderFunctor    R R (HasFunOp.idFun' _) := ⟨⟩
-    instance isEquivalenceFunctor [IsEquivalence R] : IsEquivalenceFunctor R R (HasFunOp.idFun' _) := ⟨⟩
+    instance isPreorderFunctor    [IsPreorder    R] : IsPreorderFunctor    R R (HasIdFun.idFun' _) := ⟨⟩
+    instance isEquivalenceFunctor [IsEquivalence R] : IsEquivalenceFunctor R R (HasIdFun.idFun' _) := ⟨⟩
 
   end idFun
 
   namespace constFun
 
-    variable (R : GeneralizedRelation α U) {β : U} (c : β)
+    variable {U V : Universe} [HasInstanceArrows V] [HasExternalFunctors U V]
+             [HasConstFun U V] (R : GeneralizedRelation α U) {β : V} (c : β)
 
-    def idArrow : c ⇝ c := ident (hasArrows.Arrow β) c
+    def idArrow : c ⇝ c := ident (HasInstanceArrows.Arrow β) c
 
-    instance isReflFunctor  [HasRefl  R] : IsReflFunctor  R (ConstRel α c) (HasFunOp.constFun' _ c) :=
+    instance isReflFunctor  [HasRefl  R] : IsReflFunctor  R (ConstRel α c) (HasConstFun.constFun' _ c) :=
     ⟨λ _   => idArrow c⟩
 
-    instance isSymmFunctor  [HasSymm  R] : IsSymmFunctor  R (ConstRel α c) (HasFunOp.constFun' _ c) :=
+    variable [HasInternalFunctors U] [HasFunOp V]
+
+    instance isSymmFunctor  [HasSymm  R] : IsSymmFunctor  R (ConstRel α c) (HasConstFun.constFun' _ c) :=
     ⟨λ _   => Eq.ndrec (motive := λ b : β => ⌈c ⇝ b⌉) (idArrow c) (Eq.symm (ConstRel.symmEq  α c))⟩
 
-    instance isTransFunctor [HasTrans R] : IsTransFunctor R (ConstRel α c) (HasFunOp.constFun' _ c) :=
+    instance isTransFunctor [HasTrans R] : IsTransFunctor R (ConstRel α c) (HasConstFun.constFun' _ c) :=
     ⟨λ _ _ => Eq.ndrec (motive := λ b : β => ⌈c ⇝ b⌉) (idArrow c) (Eq.symm (ConstRel.transEq α c))⟩
 
-    instance isPreorderFunctor    [IsPreorder    R] : IsPreorderFunctor    R (ConstRel α c) (HasFunOp.constFun' _ c) := ⟨⟩
-    instance isEquivalenceFunctor [IsEquivalence R] : IsEquivalenceFunctor R (ConstRel α c) (HasFunOp.constFun' _ c) := ⟨⟩
+    instance isPreorderFunctor    [IsPreorder    R] : IsPreorderFunctor    R (ConstRel α c) (HasConstFun.constFun' _ c) := ⟨⟩
+    instance isEquivalenceFunctor [IsEquivalence R] : IsEquivalenceFunctor R (ConstRel α c) (HasConstFun.constFun' _ c) := ⟨⟩
 
   end constFun
 
   namespace compFun
 
-    variable {R S T : GeneralizedRelation α U} (F : BaseFunctor R S) (G : BaseFunctor S T)
+    variable {U V W : Universe} [HasInstanceArrows V] [HasInstanceArrows W]
+             [HasExternalFunctors U V] [HasExternalFunctors V W] [HasExternalFunctors U W]
+             [HasCompFun U V W] [HasArrowCongrArg V W]
+             {R : GeneralizedRelation α U} {S : GeneralizedRelation α V} {T : GeneralizedRelation α W}
+             (F : BaseFunctor R S) (G : BaseFunctor S T)
 
     instance isReflFunctor  [HasRefl  R] [HasRefl  S] [HasRefl  T] [hF : IsReflFunctor  R S F] [hG : IsReflFunctor  S T G] :
       IsReflFunctor  R T (G ⊙' F) :=
-    ⟨λ a   => let e₁ : G (F (ident R a)) ⇝ G (ident S a) := HasFunctorialArrows.arrowCongrArg' U G (hF.respectsRefl a);
+    ⟨λ a   => let e₁ : G (F (ident R a)) ⇝ G (ident S a) := HasArrowCongrArg.arrowCongrArg G (hF.respectsRefl a);
               let e₂ : G (ident S a) ⇝ ident T a         := hG.respectsRefl a;
               HasTrans.trans' e₁ e₂⟩
 
+    variable [HasInternalFunctors U] [HasInternalFunctors V] [HasInternalFunctors W]
+
     instance isSymmFunctor  [HasSymm  R] [HasSymm  S] [HasSymm  T] [hF : IsSymmFunctor  R S F] [hG : IsSymmFunctor  S T G] :
       IsSymmFunctor  R T (G ⊙' F) :=
-    ⟨λ f   => let e₁ : G (F f⁻¹) ⇝ G (F f)⁻¹   := HasFunctorialArrows.arrowCongrArg' U G (hF.respectsSymm f);
+    ⟨λ f   => let e₁ : G (F f⁻¹) ⇝ G (F f)⁻¹   := HasArrowCongrArg.arrowCongrArg G (hF.respectsSymm f);
               let e₂ : G (F f)⁻¹ ⇝ (G (F f))⁻¹ := hG.respectsSymm (F f);
               HasTrans.trans' e₁ e₂⟩
 
     instance isTransFunctor [HasTrans R] [HasTrans S] [HasTrans T] [hF : IsTransFunctor R S F] [hG : IsTransFunctor S T G] :
       IsTransFunctor R T (G ⊙' F) :=
-    ⟨λ f g => let e₁ : G (F (g • f)) ⇝ G (F g • F f)     := HasFunctorialArrows.arrowCongrArg' U G (hF.respectsTrans f g);
+    ⟨λ f g => let e₁ : G (F (g • f)) ⇝ G (F g • F f)     := HasArrowCongrArg.arrowCongrArg G (hF.respectsTrans f g);
               let e₂ : G (F g • F f) ⇝ G (F g) • G (F f) := hG.respectsTrans (F f) (F g);
               HasTrans.trans' e₁ e₂⟩
 
@@ -496,8 +495,6 @@ section Functors
       IsEquivalenceFunctor R T (G ⊙' F) := ⟨⟩
 
   end compFun
-
-  -- TODO: HasIdFun etc.
 
 end Functors
 
@@ -528,8 +525,8 @@ section NaturalTransformations
               (nFG : ∀ a, S (mF a) (mG a))   (nGH : ∀ a, S (mG a) (mH a))
               [hnFG : IsNatural R S F G nFG] [hnGH : IsNatural R S G H nGH] :
       IsNatural R S F H (λ a => nGH a • nFG a) :=
-    ⟨λ {a b} f => let e₁ := IsCompositionRelation.applyAssocLR_left⟮IsCompositionRelation.comp_congrArg_left  (f := nFG a) (hnGH.nat f)⟯;
-                  let e₂ := IsCompositionRelation.applyAssocRL     ⟮IsCompositionRelation.comp_congrArg_right (g := nGH b) (hnFG.nat f)⟯;
+    ⟨λ {a b} f => let e₁ := IsCompositionRelation.applyAssocLR_left ⟮IsCompositionRelation.comp_congrArg_left  (f := nFG a) (hnGH.nat f)⟯;
+                  let e₂ := IsCompositionRelation.applyAssocRL      ⟮IsCompositionRelation.comp_congrArg_right (g := nGH b) (hnFG.nat f)⟯;
                   HasTrans.trans' e₁ e₂⟩
 
   end IsNaturalTransformation
